coq/LLVMGen/Correctness_GenIR.v
@@ -21,6 +21,330 @@ Opaque incLocal.
 
 Axiom int_eq_inv: forall a b, Int64.intval a ≡ Int64.intval b -> a ≡ b.
 
+Arguments add_comment /.
+Arguments add_comments /.
+Lemma wf_cfg_singleton : forall {T} (b : _ T), wf_cfg [b].
+Proof.
+  intros.
+  red.
+  eapply Coqlib.list_norepet_cons; eauto.
+  eapply Coqlib.list_norepet_nil. 
+Qed.
+
+Lemma wf_cfg_cons' : forall {T} (b : _ T) bks,
+    ¬ In (blk_id b) (map blk_id bks) ->
+    wf_cfg bks ->
+    wf_cfg (b :: bks).
+Proof.
+  intros.
+  eapply Coqlib.list_norepet_cons; eauto.
+Qed.
+
+Ltac get_block_count_hyps :=
+  repeat
+    match goal with
+    (* | H: incBlockNamed ?n ?s1 ≡ inr (?s2, _) |- _ => *)
+      (* apply incBlockNamed_block_count in H *)
+    (* | H: incLocalNamed ?n ?s1 ≡ inr (?s2, _) |- _ => *)
+    (* apply incLocalNamed_block_count in H *)
+    | H: resolve_PVar _ _ ≡ _ |- _ => apply resolve_PVar_state in H
+    | H: incVoid ?s1 ≡ inr (?s2, _) |- _ =>
+      apply incVoid_block_count in H
+    | H: incLocal ?s1 ≡ inr (?s2, _) |- _ =>
+      apply incLocal_block_count in H
+    | H : genNExpr _ _ ≡ inr _ |- _ =>
+      apply genNExpr_local_count in H
+    | H: genMExpr ?m ?s1 ≡ inr (?s2, _) |- _ =>
+      apply genMExpr_block_count in H
+    | H: genAExpr ?a ?s1 ≡ inr (?s2, _) |- _ =>
+      apply genAExpr_block_count in H
+    | H: genIR ?op ?id ?s1 ≡ inr (?s2, _) |- _ =>
+      apply genIR_block_count in H
+    end.
+
+
+Transparent incBlockNamed.
+Lemma foo :
+  ∀ (op : DSHOperator) (s1 s2 : IRState) (nextblock b : block_id) (bk_op : list (LLVMAst.block typ)),
+    bid_bound s1 nextblock ->
+    genIR op nextblock s1 ≡ inr (s2, (b, bk_op)) →
+    wf_cfg bk_op. 
+Proof.
+  induction op; intros * NEXT GEN.
+  - cbn* in *; simp; cbn.
+    eapply wf_cfg_singleton.
+  - cbn* in *; simp; cbn in *.
+    eapply wf_cfg_singleton.
+  - destruct NEXT as (? & [?bid ? ? ?] & [?bid ? ? ?] & ? & ? & ?).
+    cbn* in *.
+    simp.
+    cbn* in *; simp; cbn in *.
+    clean_goal.
+    get_block_count_hyps; subst; cbn in *.
+    repeat match goal with
+           | h: IRState |- _ => destruct h as [?bid ? ? ?]
+           end; cbn in *.
+    subst.
+    eapply wf_cfg_cons'.
+    { cbn.
+      intuition;
+        match goal with
+        | h: Name _ ≡ Name _ |- _ => apply Name_inj in h; inv h
+        end. 
+    }
+    eapply wf_cfg_cons'.
+    { cbn.
+      intuition;
+        match goal with
+        | h: Name _ ≡ Name _ |- _ => apply Name_inj in h; inv h
+        end. 
+    }
+    eapply wf_cfg_cons'.
+    { cbn.
+      intuition;
+        match goal with
+        | h: Name _ ≡ Name _ |- _ => apply Name_inj in h; inv h
+        end. 
+    }
+    eapply wf_cfg_singleton.
+  - destruct NEXT as (? & [?bid ? ? ?] & [?bid ? ? ?] & ? & ? & ?).
+    cbn* in *.
+    simp.
+    cbn* in *; simp; cbn in *.
+    clean_goal.
+    get_block_count_hyps; subst; cbn in *.
+    repeat match goal with
+           | h: IRState |- _ => destruct h as [?bid ? ? ?]
+           end; cbn in *.
+    subst.
+    eapply wf_cfg_cons'.
+    { cbn.
+      intuition;
+        match goal with
+        | h: Name _ ≡ Name _ |- _ => apply Name_inj in h; inv h
+        end. 
+    }
+    eapply wf_cfg_cons'.
+    { cbn.
+      intuition;
+        match goal with
+        | h: Name _ ≡ Name _ |- _ => apply Name_inj in h; inv h
+        end. 
+    }
+    eapply wf_cfg_cons'.
+    { cbn.
+      intuition;
+        match goal with
+        | h: Name _ ≡ Name _ |- _ => apply Name_inj in h; inv h
+        end. 
+    }
+    eapply wf_cfg_singleton.
+
+  - destruct NEXT as (? & [?bid ? ? ?] & [?bid ? ? ?] & ? & ? & ?).
+    cbn* in *.
+    simp.
+    cbn* in *; simp; cbn in *.
+    clean_goal.
+    get_block_count_hyps; subst; cbn in *.
+    repeat match goal with
+           | h: IRState |- _ => destruct h as [?bid ? ? ?]
+           end; cbn in *.
+    subst.
+    eapply wf_cfg_cons'.
+    { cbn.
+      intuition;
+        match goal with
+        | h: Name _ ≡ Name _ |- _ => apply Name_inj in h; inv h
+        end. 
+    }
+    eapply wf_cfg_cons'.
+    { cbn.
+      intuition;
+        match goal with
+        | h: Name _ ≡ Name _ |- _ => apply Name_inj in h; inv h
+        end. 
+    }
+    eapply wf_cfg_cons'.
+    { cbn.
+      intuition;
+        match goal with
+        | h: Name _ ≡ Name _ |- _ => apply Name_inj in h; inv h
+        end. 
+    }
+    eapply wf_cfg_singleton.
+
+  - destruct NEXT as (? & [?bid ? ? ?] & [?bid ? ? ?] & ? & ? & ?).
+    cbn* in *.
+    simp.
+    cbn* in *; simp; cbn in *.
+    clean_goal.
+    get_block_count_hyps; subst; cbn in *.
+    repeat match goal with
+           | h: IRState |- _ => destruct h as [?bid ? ? ?]
+           end; cbn in *.
+    subst.
+    eapply wf_cfg_cons'.
+    { cbn.
+      intuition;
+        match goal with
+        | h: Name _ ≡ Name _ |- _ => apply Name_inj in h; inv h
+        end. 
+    }
+    eapply wf_cfg_cons'.
+    { cbn.
+      intuition;
+        match goal with
+        | h: Name _ ≡ Name _ |- _ => apply Name_inj in h; inv h
+        end. 
+    }
+    eapply wf_cfg_cons'.
+    { cbn.
+      intuition;
+        match goal with
+        | h: Name _ ≡ Name _ |- _ => apply Name_inj in h; inv h
+        end. 
+    }
+    eapply wf_cfg_singleton.
+
+  - simpl in *.
+    pose (incBlockNamed "Loop_lcont" s1).
+
+    (* assert (ALPHA: not_ends_with_nat "Loop_lcont") by admit. *)
+    pose proof bid_bound_incBlockNamed
+    cbn in s.
+    
+    assert (bid_bound s1 (Name ("Loop_lcont" @@ string_of_nat (block_count s1)))).
+    {
+      eapply bid_bound_incBlockNamed with (s1 := s1). [| reflexivity].     
+      }
+    destruct NEXT as (? & [?bid ? ? ?] & [?bid ? ? ?] & ? & ? & ?).
+    cbn* in *.
+    simp.
+    eapply IHop in Heqs0.
+    2:{
+      eapply bid_bound_incLocal_mono.
+      eapply bid_bound_incBlockNamed with (s1 := s1) (name := "loop_lcont").
+      2:cbn.
+     
+    cbn* in *; simp; cbn in *.
+
+    clean_goal.
+    get_block_count_hyps; subst; cbn in *.
+    repeat match goal with
+           | h: IRState |- _ => destruct h as [?bid ? ? ?]
+           end; cbn in *.
+    subst.
+    eapply wf_cfg_cons'.
+    { cbn.
+      intuition;
+        match goal with
+        | h: Name _ ≡ Name _ |- _ => apply Name_inj in h; inv h
+        end. 
+    }
+    eapply wf_cfg_cons'.
+    { cbn.
+      intuition;
+        match goal with
+        | h: Name _ ≡ Name _ |- _ => apply Name_inj in h; inv h
+        end. 
+    }
+    eapply wf_cfg_cons'.
+    { cbn.
+      intuition;
+        match goal with
+        | h: Name _ ≡ Name _ |- _ => apply Name_inj in h; inv h
+        end. 
+    }
+    eapply wf_cfg_singleton.
+
+  - destruct NEXT as (? & [?bid ? ? ?] & [?bid ? ? ?] & ? & ? & ?).
+    cbn* in *.
+    simp.
+    cbn* in *; simp; cbn in *.
+    clean_goal.
+    get_block_count_hyps; subst; cbn in *.
+    repeat match goal with
+           | h: IRState |- _ => destruct h as [?bid ? ? ?]
+           end; cbn in *.
+    subst.
+    eapply wf_cfg_cons'.
+    { cbn.
+      intuition;
+        match goal with
+        | h: Name _ ≡ Name _ |- _ => apply Name_inj in h; inv h
+        end. 
+    }
+    eapply wf_cfg_cons'.
+    { cbn.
+      intuition;
+        match goal with
+        | h: Name _ ≡ Name _ |- _ => apply Name_inj in h; inv h
+        end. 
+    }
+    eapply wf_cfg_cons'.
+    { cbn.
+      intuition;
+        match goal with
+        | h: Name _ ≡ Name _ |- _ => apply Name_inj in h; inv h
+        end. 
+    }
+    eapply wf_cfg_singleton.
+
+  - destruct NEXT as (? & [?bid ? ? ?] & [?bid ? ? ?] & ? & ? & ?).
+    cbn* in *.
+    simp.
+    cbn* in *; simp; cbn in *.
+    clean_goal.
+    get_block_count_hyps; subst; cbn in *.
+    repeat match goal with
+           | h: IRState |- _ => destruct h as [?bid ? ? ?]
+           end; cbn in *.
+    subst.
+    eapply wf_cfg_cons'.
+    { cbn.
+      intuition;
+        match goal with
+        | h: Name _ ≡ Name _ |- _ => apply Name_inj in h; inv h
+        end. 
+    }
+    eapply wf_cfg_cons'.
+    { cbn.
+      intuition;
+        match goal with
+        | h: Name _ ≡ Name _ |- _ => apply Name_inj in h; inv h
+        end. 
+    }
+    eapply wf_cfg_cons'.
+    { cbn.
+      intuition;
+        match goal with
+        | h: Name _ ≡ Name _ |- _ => apply Name_inj in h; inv h
+        end. 
+    }
+    eapply wf_cfg_singleton.
+
+
+
+      2:eapply wf_cfg_cons'.
+      3:eapply wf_cfg_cons'.
+      4:
+      all:cbn.
+      clean_goal.
+      intuition.
+      subst.
+      cbn in *.
+      subst.
+
+    cbn in *.
+    rewrite Heqs in *; clear Heqs.
+
+    assert (b <> b0).
+
+    
+Opaque incBlockNamed.
+
+
+
 Section GenIR.
 
   (* The result is a branch *)
@@ -375,18 +699,20 @@ Section GenIR.
     - rewrite EQ; apply MINV.
     - red. rewrite EQ; apply WF.
   Qed.
+
   
+
   Lemma compile_FSHCOL_correct :
     forall (** Compiler bits *) (s1 s2: IRState)
       (** Helix bits    *) (op: DSHOperator) (σ : evalContext) (memH : memoryH) 
       (** Vellvm bits   *) (nextblock bid_in bid_from : block_id) (bks : list (LLVMAst.block typ))
       (* (env : list (ident * typ)) *)  (g : global_env) ((* ρi  *)ρ : local_env) (memV : memoryV),
       bid_bound s1 nextblock ->
-      (GenIR_Rel σ s1 bid_in (* ⩕ lift_Rel_cfg (fresh_pre s1 s2) *)) (memH,tt) (memV, (ρ, (g, (inl (bid_from, bid_in))))) ->
+      (GenIR_Rel σ s1 bid_in) (memH,tt) (memV, (ρ, (g, (inl (bid_from, bid_in))))) ->
       Gamma_safe σ s1 s2 ->
       no_failure (E := E_cfg) (interp_helix (denoteDSHOperator σ op) memH) -> (* Evaluation succeeds *)
       genIR op nextblock s1 ≡ inr (s2,(bid_in,bks)) ->
-      eutt (succ_cfg (GenIR_Rel σ s2 nextblock (* ⩕ lift_Rel_cfg (fresh_post s1 s2 ρ) *)))
+      eutt (succ_cfg (GenIR_Rel σ s2 nextblock))
            (interp_helix (denoteDSHOperator σ op) memH)
            (interp_cfg (D.denote_bks (convert_typ [] bks) (bid_from,bid_in))
                        g ρ memV).
